Progress in termination proofs

ConstantPropagationAnalysis.v
@@ -305,42 +305,6 @@ Instance set_var_semilattice : BoundedSemiLattice Dom := {
 Qed.
 
 
-  Fixpoint list_update_at {X} (L:list X) (n:nat) (v:X)  :=
-    match L, n with
-      | x::L, 0 => v::L
-      | x::L, S n => x::list_update_at L n v
-      | _, _ => nil
-    end.
-
-  Lemma list_update_at_length X (l:list X) off v
-  : length (list_update_at l off v) = length l.
-  Proof.
-    general induction l; simpl; eauto.
-    - destruct off; simpl; eauto.
-  Qed.
-
-  Lemma list_update_at_get_1 X (l:list X) off v v' n
-  : get (list_update_at l off v') n v
-    -> n <> off
-    -> get l n v.
-  Proof.
-    intros. general induction l; simpl in * |- *; isabsurd.
-    - destruct off; simpl in *.
-      * inv H; intuition.
-      * inv H; intuition (eauto using get).
-  Qed.
-
-  Lemma list_update_at_get_2 X (l:list X) off v v' n
-  : get (list_update_at l off v') n v
-    -> n = off
-    -> v = v'.
-  Proof.
-    intros.
-    general induction H; simpl in * |- *; isabsurd.
-    - destruct l; simpl in *; isabsurd; congruence.
-    - destruct l; simpl in *; isabsurd.
-      inv Heql0; eauto.
-  Qed.
 
 Definition domupd (d:Dom) x (o:option val) : Dom :=
   match o with
