Libs/PartialOrder.v
@@ -2,18 +2,43 @@ Require Import Util LengthEq.
 Require Import Containers.OrderedType Setoid Coq.Classes.Morphisms Computable
         Coq.Classes.RelationClasses.
 Require Import Containers.OrderedTypeEx DecSolve MoreList OrderedTypeEx.
+Require Import AllInRel.
 
 Class PartialOrder (Dom:Type) := {
   poLe : Dom -> Dom -> Prop;
   poLe_dec :> forall d d', Computable (poLe d d');
   poEq : Dom -> Dom -> Prop;
   poEq_dec :> forall d d', Computable (poEq d d');
-  poEq_refl : forall d d', poEq d d' -> poLe d d';
   poEq_equivalence :> Equivalence poEq;
-  po_antisymmetric :> Antisymmetric _ poEq poLe;
+  poLe_refl : forall d d', poEq d d' -> poLe d d';
+  poLe_trans :> Transitive poLe;
+  poLe_antisymmetric :> Antisymmetric _ poEq poLe;
 }.
 
+Instance PartialOrder_poLe_refl Dom `{PartialOrder Dom} : Reflexive poLe.
+Proof.
+  hnf; intros. eapply poLe_refl. reflexivity.
+Qed.
+
 Definition poLt {Dom} `{PartialOrder Dom} x y := poLe x y /\ ~ poEq x y.
+
+Lemma poLt_intro Dom `{PartialOrder Dom} x y
+  : poLe x y -> ~ poEq x y -> poLt x y.
+Proof.
+  firstorder.
+Qed.
+
+Lemma poLt_poLe Dom `{PartialOrder Dom} x y
+  : poLt x y -> poLe x y.
+Proof.
+  firstorder.
+Qed.
+
+Hint Resolve poLt_intro poLt_poLe.
+
+Notation "s '⊑' t" := (poLe s t) (at level 70, no associativity).
+Notation "s '⊏' t" := (poLt s t) (at level 70, no associativity).
+Notation "s '≣' t" := (poEq s t) (at level 70, no associativity).
 
 Instance PartialOrder_pair_instance X `{PartialOrder X} Y `{PartialOrder Y}
 : PartialOrder (X * Y) := {
@@ -23,12 +48,13 @@ Instance PartialOrder_pair_instance X `{PartialOrder X} Y `{PartialOrder Y}
   poEq_dec := _
 }.
 Proof.
-  - intros; dcr; split; eapply poEq_refl; eauto.
   - econstructor.
     + hnf; intros; split; reflexivity.
     + hnf; intros; dcr; split; symmetry; eauto.
     + hnf; intros; dcr; split; etransitivity; eauto.
-  - intros. dcr; split; eapply po_antisymmetric; eauto.
+  - intros; dcr; split; eapply poLe_refl; eauto.
+  - hnf; intros; dcr; split; etransitivity; eauto.
+  - hnf; intros; dcr; split; eapply poLe_antisymmetric; eauto.
 Defined.
 
 Instance PartialOrder_list_instance X `{PartialOrder X}
@@ -39,8 +65,70 @@ Instance PartialOrder_list_instance X `{PartialOrder X}
   poEq_dec := _
 }.
 Proof.
-  - intros. general induction H0; eauto using @list_eq, poEq_refl.
+  - intros. general induction H0; eauto using @list_eq, poLe_refl.
+  - intros ? ? ? R1 R2.
+    general induction R1; inv R2; eauto using @list_eq, poLe_trans.
   - intros ? ? EQ1 EQ2.
     exploit list_eq_length as LEN; eauto. length_equify.
-    general induction LEN; inv EQ1; inv EQ2; eauto using @list_eq, po_antisymmetric.
+    general induction LEN; inv EQ1; inv EQ2; eauto using @list_eq, poLe_antisymmetric.
+Defined.
+
+Instance poLe_poEq_impl Dom `{PartialOrder Dom}
+  : Proper (poEq ==> poEq ==> impl) poLe.
+Proof.
+  unfold Proper, respectful, impl; intros.
+  symmetry in H0.
+  - eapply poLe_refl in H0. eapply poLe_refl in H1.
+    etransitivity; eauto. etransitivity; eauto.
+Qed.
+
+Instance poLe_poEq_flip_impl Dom `{PartialOrder Dom}
+  : Proper (poEq ==> poEq ==> flip impl) poLe.
+Proof.
+  unfold Proper, respectful, flip, impl; intros.
+  - eapply poLe_refl in H0. symmetry in H1. eapply poLe_refl in H1.
+    etransitivity; eauto. etransitivity; eauto.
+Qed.
+
+Instance poLe_poEq_iff Dom `{PartialOrder Dom}
+  : Proper (poEq ==> poEq ==> iff) poLe.
+Proof.
+  unfold Proper, respectful, impl; intros.
+  split; intros.
+  - rewrite <- H0. rewrite H2. eauto using poLe_refl.
+  - rewrite H0. rewrite H1. eauto using poLe_refl.
+Qed.
+
+Instance poLt_poLe_impl Dom `{PartialOrder Dom}
+  : Proper (flip poLe ==> poLe ==> impl) poLt.
+Proof.
+  unfold Proper, respectful, flip, impl; intros.
+  destruct H2. split; intros.
+  - etransitivity; eauto. etransitivity; eauto.
+  - intro. eapply H3. eapply poLe_antisymmetric; eauto.
+    etransitivity; eauto. rewrite <- H4. eauto.
+Qed.
+
+Instance poLt_poLe_flip_impl Dom `{PartialOrder Dom}
+  : Proper (poLe ==> flip poLe ==> flip impl) poLt.
+Proof.
+  unfold Proper, respectful, flip, impl; intros.
+  destruct H2. split; intros.
+  - etransitivity; eauto. etransitivity; eauto.
+  - intro. eapply H3. eapply poLe_antisymmetric; eauto.
+    etransitivity; eauto. rewrite <- H4. eauto.
+Qed.
+
+
+
+Instance PartialOrder_ann Dom `{PartialOrder Dom}
+: PartialOrder (list Dom) := {
+  poLe := PIR2 poLe;
+  poLe_dec := @PIR2_computable _ _ poLe poLe_dec;
+  poEq := PIR2 poEq;
+  poEq_dec := @PIR2_computable _ _ poEq poEq_dec;
+}.
+Proof.
+  - intros. general induction H0; eauto using @PIR2, poLe_refl.
+  - intros ? ? A B. general induction A; inv B; eauto 20 using @PIR2, poLe_antisymmetric.
 Defined.
