Equiv/ProofRelations.v
@@ -1,4 +1,4 @@
-Require Import Util paco.
+Require Import Util paco2.
 Require Import Env Var SmallStepRelations StateType IL InRel Equiv.
 
 (* A proof relation is parameterized by analysis information A *)
