Infra/ListUpdateAt.v
@@ -1,0 +1,46 @@
+Require Import Util Get.
+
+Fixpoint list_update_at {X} (L:list X) (n:nat) (v:X)  :=
+  match L, n with
+  | x::L, 0 => v::L
+  | x::L, S n => x::list_update_at L n v
+  | _, _ => nil
+  end.
+
+Lemma list_update_at_length X (l:list X) off v
+  : length (list_update_at l off v) = length l.
+Proof.
+  general induction l; simpl; eauto.
+  - destruct off; simpl; eauto.
+Qed.
+
+Lemma list_update_at_get_1 X (l:list X) off v v' n
+  : get (list_update_at l off v') n v
+    -> n <> off
+    -> get l n v.
+Proof.
+  intros. general induction l; simpl in * |- *; isabsurd.
+  - destruct off; simpl in *.
+    * inv H; intuition.
+    * inv H; intuition (eauto using get).
+Qed.
+
+Lemma list_update_at_get_2 X (l:list X) off v v' n
+  : get (list_update_at l off v') n v
+    -> n = off
+    -> v = v'.
+Proof.
+  intros.
+  general induction H; simpl in * |- *; isabsurd.
+  - destruct l; simpl in *; isabsurd; congruence.
+  - destruct l; simpl in *; isabsurd.
+    inv Heql0; eauto.
+Qed.
+
+Lemma list_update_at_get_3 X (l:list X) v' v n
+  : get l n v'
+    -> get (list_update_at l n v) n v.
+Proof.
+  intros Get.
+  general induction Get; simpl in * |- *; eauto with get.
+Qed.
